Add live variables to reds relation, finish Application case of correctness proof

Launchbury.thy
@@ -2,13 +2,6 @@ theory Launchbury
 imports Terms Heap
 begin
 
-lemma fresh_delete:
-  assumes "atom x \<sharp> \<Gamma>"
-  shows "atom x \<sharp> \<Gamma>(y := None)"
-apply (simp add: fresh_def)
-apply (simp add: supp_def)
-oops
-
 lemma fresh_remove:
   assumes "atom x \<sharp> \<Gamma>"
   shows "atom x \<sharp> (removeAll e \<Gamma>)"
@@ -31,12 +24,12 @@ by(induct e y z and as y z rule:subst_subst_assn.induct)
   (auto simp add:exp_assn.fresh fresh_at_base fresh_star_Pair exp_assn.bn_defs fresh_star_insert)
 
 
-inductive reds :: "heap \<Rightarrow> exp \<Rightarrow> heap \<Rightarrow> exp \<Rightarrow> bool" ("_ : _ \<Down> _ : _" [50,50,50,50] 50)
+inductive reds :: "heap \<Rightarrow> exp \<Rightarrow> var list \<Rightarrow> heap \<Rightarrow> exp \<Rightarrow> bool" ("_ : _ \<Down>\<^bsub>_\<^esub> _ : _" [50,50,50,50] 50)
 where
-  Lambda: "\<Gamma> : (Lam [x]. e) \<Down> \<Gamma> : (Lam [x]. e)" 
- | Application: "\<lbrakk> atom y \<sharp> (\<Gamma>,e,x,\<Delta>,\<Theta>,z) ; \<Gamma> : e \<Down> \<Delta> : (Lam [y]. e') ; \<Delta> : e'[y ::= x] \<Down> \<Theta> : z\<rbrakk> \<Longrightarrow> \<Gamma> : App e x \<Down> \<Theta> : z" 
- | Variable: "\<lbrakk> (x,e) \<in> set \<Gamma>; removeAll (x, e) \<Gamma> : e \<Down> \<Delta> : z \<rbrakk> \<Longrightarrow> \<Gamma> : Var x \<Down> (x, z) # \<Delta> : z"
- | Let: "asToHeap as @ \<Gamma> : body \<Down> \<Delta> : z \<Longrightarrow> \<Gamma> : Let as body \<Down> \<Delta> : z"
+  Lambda: "\<Gamma> : (Lam [x]. e) \<Down>\<^bsub>L\<^esub> \<Gamma> : (Lam [x]. e)" 
+ | Application: "\<lbrakk> atom y \<sharp> (\<Gamma>,e,x,L,\<Delta>,\<Theta>,z) ; \<Gamma> : e \<Down>\<^bsub>x#L\<^esub> \<Delta> : (Lam [y]. e') ; \<Delta> : e'[y ::= x] \<Down>\<^bsub>L\<^esub> \<Theta> : z\<rbrakk> \<Longrightarrow> \<Gamma> : App e x \<Down>\<^bsub>L\<^esub> \<Theta> : z" 
+ | Variable: "\<lbrakk> (x,e) \<in> set \<Gamma>; removeAll (x, e) \<Gamma> : e \<Down>\<^bsub>L\<^esub> \<Delta> : z \<rbrakk> \<Longrightarrow> \<Gamma> : Var x \<Down>\<^bsub>L\<^esub> (x, z) # \<Delta> : z"
+ | Let: "set (bn as) \<sharp>* L \<Longrightarrow> asToHeap as @ \<Gamma> : body \<Down>\<^bsub>L\<^esub> \<Delta> : z \<Longrightarrow> \<Gamma> : Let as body \<Down>\<^bsub>L\<^esub> \<Delta> : z"
 
 equivariance reds
 
@@ -51,19 +44,19 @@ apply (auto simp add: fresh_star_def fresh_Pair exp_assn.fresh)
 done
 
 lemma eval_test:
-  "[] : (Let (ACons x (Lam [y]. Var y) ANil) (Var x)) \<Down> [(x, Lam [y]. Var y)] : (Lam [y]. Var y)"
+  "[] : (Let (ACons x (Lam [y]. Var y) ANil) (Var x)) \<Down>\<^bsub>[]\<^esub> [(x, Lam [y]. Var y)] : (Lam [y]. Var y)"
 apply(auto intro!: Lambda Application Variable Let
- simp add: fresh_Pair fresh_Cons fresh_Nil exp_assn.fresh)
+ simp add: fresh_Pair fresh_Cons fresh_Nil exp_assn.fresh fresh_star_def)
 done
 
 lemma eval_test2:
-  "y \<noteq> x \<Longrightarrow> [] : (Let (ACons x (Lam [y]. Var y) ANil) (App (Var x) x)) \<Down> [(x, Lam [y]. Var y)] : (Lam [y]. Var y)"
-by (auto intro!: Lambda Application Variable Let simp add: fresh_Pair fresh_at_base fresh_Cons fresh_Nil exp_assn.fresh)
+  "y \<noteq> x \<Longrightarrow> [] : (Let (ACons x (Lam [y]. Var y) ANil) (App (Var x) x)) \<Down>\<^bsub>[]\<^esub> [(x, Lam [y]. Var y)] : (Lam [y]. Var y)"
+by (auto intro!: Lambda Application Variable Let simp add: fresh_Pair fresh_at_base fresh_Cons fresh_Nil exp_assn.fresh fresh_star_def)
 
 lemma reds_doesnt_forget:
-  "\<Gamma> : e \<Down> \<Delta> : z \<Longrightarrow> heapVars \<Gamma> \<subseteq> heapVars \<Delta>"
+  "\<Gamma> : e \<Down>\<^bsub>L\<^esub> \<Delta> : z \<Longrightarrow> heapVars \<Gamma> \<subseteq> heapVars \<Delta>"
 proof(induct rule: reds.induct)
-case(Variable v e \<Gamma> \<Delta> z)
+case(Variable v e \<Gamma> L \<Delta> z)
   show ?case
   proof
     fix x
@@ -74,7 +67,6 @@ case(Variable v e \<Gamma> \<Delta> z)
       thus ?thesis by simp
     next
     case False
-      print_facts
       with `x \<in> heapVars \<Gamma>`
       have "x \<in> heapVars (removeAll (v,e) \<Gamma>)" by (auto simp add: heapVars_def)
       hence "x \<in> heapVars \<Delta>" using Variable.hyps(3) by auto
@@ -83,14 +75,40 @@ case(Variable v e \<Gamma> \<Delta> z)
   qed
 qed (auto)
 
+lemma reds_avoids_live:
+  "\<lbrakk> \<Gamma> : e \<Down>\<^bsub>L\<^esub> \<Delta> : z;
+   x \<in> set L;
+   x \<notin> heapVars \<Gamma>
+  \<rbrakk> \<Longrightarrow> x \<notin> heapVars \<Delta>"
+proof(induct rule:reds.induct)
+case (Lambda \<Gamma> x e L) thus ?case by auto
+next
+case (Application y \<Gamma> e x L \<Delta> \<Theta> z e') thus ?case by auto
+next
+case (Variable  x e \<Gamma> L \<Delta> z) thus ?case by (auto simp add: heapVars_def, metis fst_conv imageI)
+next
+case (Let as L \<Gamma> body \<Delta> z)
+  print_facts
+  have "x \<notin> heapVars \<Gamma>" by fact moreover
+  have "x \<notin> heapVars (asToHeap as)"
+    using `set (bn as) \<sharp>* L` and `x \<in> set L`
+    apply -
+    apply (induct as rule: asToHeap.induct)
+    apply (auto simp add: exp_assn.bn_defs fresh_star_insert)
+    by (metis finite_set fresh_finite_set_at_base fresh_set)  ultimately
+  have "x \<notin> heapVars (asToHeap as @ \<Gamma>)" by (auto simp del:fst_set_asToHeap)  
+  thus ?case
+    by (rule Let.hyps(3)[OF `x \<in> set L`])
+qed
 
-lemma reds_fresh:" \<lbrakk> \<Gamma> : e \<Down> \<Delta> : z;
+
+lemma reds_fresh:" \<lbrakk> \<Gamma> : e \<Down>\<^bsub>L\<^esub> \<Delta> : z;
    atom (x::var) \<sharp> (\<Gamma>, e)
   \<rbrakk> \<Longrightarrow> atom x \<sharp> (\<Delta>, z) \<or> x \<in> heapVars \<Delta>"
 proof(induct rule: reds.induct)
 case (Lambda \<Gamma> x e) thus ?case by auto
 next
-case (Application y \<Gamma> e x' \<Delta> \<Theta> z e')
+case (Application y \<Gamma> e x' L \<Delta> \<Theta> z e')
   hence "atom x \<sharp> (\<Delta>, Lam [y]. e') \<or> x \<in> heapVars \<Delta>" by (auto simp add: exp_assn.fresh fresh_Pair)
 
   thus ?case
@@ -116,14 +134,14 @@ case (Application y \<Gamma> e x' \<Delta> \<Theta> z e')
   qed
 next
 
-case(Variable v e \<Gamma> \<Delta> z)
+case(Variable v e \<Gamma> L \<Delta> z)
   have "atom x \<sharp> \<Gamma>" and "atom x \<sharp> v" using Variable.prems(1) by (auto simp add: fresh_Pair exp_assn.fresh)
   hence "atom x \<sharp> removeAll (v,e) \<Gamma>" and "atom x \<sharp> e" using `(v,e) \<in> set \<Gamma>` by(auto intro: fresh_remove dest:fresh_list_elem)
   hence "atom x \<sharp> (\<Delta>, z) \<or> x \<in> heapVars \<Delta>"  using Variable.hyps(3) by (auto simp add: fresh_Pair)
   thus ?case using `atom x \<sharp> v` by (auto simp add: fresh_Pair fresh_Cons fresh_at_base)
 next
 
-case (Let as \<Gamma> body \<Delta> z)
+case (Let as \<Gamma> body L \<Delta> z)
   show ?case
     proof (cases "atom x \<in> set(bn as)")
     case False
@@ -131,14 +149,14 @@ case (Let as \<Gamma> body \<Delta> z)
       hence "atom x \<sharp> asToHeap as"
         by(induct as rule:asToHeap_induct)(auto simp add: fresh_Nil fresh_Cons fresh_Pair exp_assn.fresh)
       show ?thesis
-        apply(rule Let.hyps(2))
+        apply(rule Let.hyps(3))
         using Let.prems `atom x \<sharp> asToHeap as` False
         by (auto simp add: fresh_Pair exp_assn.fresh fresh_append)
     next
     case True
       hence "x \<in> heapVars (asToHeap as)" 
         by(induct as rule:asToHeap_induct)(auto simp add: exp_assn.bn_defs)      
-      thus ?thesis using reds_doesnt_forget[OF Let.hyps(1)] by auto
+      thus ?thesis using reds_doesnt_forget[OF Let.hyps(2)] by auto
     qed
 qed
 
