Correctness.thy
@@ -2,9 +2,25 @@ theory Correctness
   imports Denotational Launchbury
 begin
 
+lemma preserve_meaning:
+  assumes "\<Gamma> : e \<Down>\<^bsub>L\<^esub> \<Delta> : z"
+  and "x \<in> set L"
+  and "\<lbrace>\<Gamma>\<rbrace>\<rho> \<le> \<lbrace>\<Delta>\<rbrace>\<rho>"
+  shows "\<lbrakk>Var x\<rbrakk>\<^bsub>\<lbrace>\<Gamma>\<rbrace>\<rho>\<^esub> = \<lbrakk>Var x\<rbrakk>\<^bsub>\<lbrace>\<Delta>\<rbrace>\<rho>\<^esub>"
+proof(cases "x \<in> heapVars \<Gamma>")
+case True
+  thus ?thesis
+  using fmap_less_eqD[OF `\<lbrace>\<Gamma>\<rbrace>\<rho> \<le> \<lbrace>\<Delta>\<rbrace>\<rho>`, of x] 
+  by (auto simp add: heapVars_def)
+next
+case False with reds_avoids_live[OF assms(1,2)]
+  have "\<lbrakk>Var x\<rbrakk>\<^bsub>\<lbrace>\<Gamma>\<rbrace>\<rho>\<^esub> = the (lookup \<rho> x)" and "\<lbrakk>Var x\<rbrakk>\<^bsub>\<lbrace>\<Delta>\<rbrace>\<rho>\<^esub> = the (lookup \<rho> x)"
+    by (auto intro:  the_lookup_HSem_other simp add: heapVars_def)
+  thus ?thesis by simp
+qed
 
 theorem correctness:
-  assumes "\<Gamma> : e \<Down> \<Delta> : z"
+  assumes "\<Gamma> : e \<Down>\<^bsub>L\<^esub> \<Delta> : z"
   shows "\<lbrakk>e\<rbrakk>\<^bsub>\<lbrace>\<Gamma>\<rbrace>\<rho>\<^esub> = \<lbrakk>z\<rbrakk>\<^bsub>\<lbrace>\<Delta>\<rbrace>\<rho>\<^esub>" and "\<lbrace>\<Gamma>\<rbrace>\<rho> \<le> \<lbrace>\<Delta>\<rbrace>\<rho>"
   using assms
 proof(nominal_induct avoiding: \<rho>  rule:reds.strong_induct)
@@ -13,13 +29,13 @@ case (Lambda \<Gamma> x e)
   case 1 show ?case by simp
   case 2 show ?case by simp
 next
-case (Application y \<Gamma> e x \<Delta> \<Theta> z e') case 1
+case (Application y \<Gamma> e x L \<Delta> \<Theta> z e') case 1
   have "\<lbrakk> App e x \<rbrakk>\<^bsub>\<lbrace>\<Gamma>\<rbrace>\<rho>\<^esub> = \<lbrakk> e \<rbrakk>\<^bsub>\<lbrace>\<Gamma>\<rbrace>\<rho>\<^esub> \<down>Fn \<lbrakk> Var x \<rbrakk>\<^bsub>\<lbrace>\<Gamma>\<rbrace>\<rho>\<^esub>"
     by simp also
   have "... = \<lbrakk> Lam [y]. e' \<rbrakk>\<^bsub>\<lbrace>\<Delta>\<rbrace>\<rho>\<^esub> \<down>Fn \<lbrakk> Var x \<rbrakk>\<^bsub>\<lbrace>\<Gamma>\<rbrace>\<rho>\<^esub>"
     using `\<lbrakk> e \<rbrakk>\<^bsub>\<lbrace>\<Gamma>\<rbrace>\<rho>\<^esub> = _` by simp also
   have "... = \<lbrakk> Lam [y]. e' \<rbrakk>\<^bsub>\<lbrace>\<Delta>\<rbrace>\<rho>\<^esub> \<down>Fn \<lbrakk> Var x \<rbrakk>\<^bsub>\<lbrace>\<Delta>\<rbrace>\<rho>\<^esub>"
-    sorry also
+    by (subst preserve_meaning[OF `\<Gamma> : e \<Down>\<^bsub>x # L\<^esub> \<Delta> : Lam [y]. e'` _ `\<lbrace>\<Gamma>\<rbrace>\<rho> \<le> \<lbrace>\<Delta>\<rbrace>\<rho>`], auto) also
   have "... = (\<Lambda> v. \<lbrakk> e' \<rbrakk>\<^bsub>(\<lbrace>\<Delta>\<rbrace>\<rho>)(y f\<mapsto> v)\<^esub>)\<cdot>(\<lbrakk> Var x \<rbrakk>\<^bsub>\<lbrace>\<Delta>\<rbrace>\<rho>\<^esub>)"
     using `atom y \<sharp> \<Delta>` and `atom y \<sharp> \<rho>` by simp also
   have "... = \<lbrakk> e' \<rbrakk>\<^bsub>(\<lbrace>\<Delta>\<rbrace>\<rho>)(y f\<mapsto> (\<lbrakk> Var x \<rbrakk>\<^bsub>\<lbrace>\<Delta>\<rbrace>\<rho>\<^esub>))\<^esub>"
